src/program_proof/grove_shared/urpc_proof.v
@@ -162,7 +162,7 @@ Definition Client_lock_inner Γ  (cl : loc) (lk : loc) mref : iProp Σ :=
             "Hmapping_ctx" ∷ map_ctx (ccmapping_name Γ) 1 reqs ∗
             "Hescrow_ctx" ∷ map_ctx (ccescrow_name Γ) 1 estoks ∗
             "Hextracted_ctx" ∷ map_ctx (ccextracted_name Γ) 1 extoks ∗
-            "Hpending_map" ∷ map.is_map mref 1 (pending, zero_val ptrT) ∗
+            "Hpending_map" ∷ map.own_map mref 1 (pending, zero_val ptrT) ∗
             "Hreqs" ∷ [∗ map] seqno ↦ req ∈ reqs,
                  ∃ (Post : list u8 → iProp Σ),
                  "Hreg_entry" ∷  ptsto_ro (ccmapping_name Γ) seqno req ∗
@@ -206,12 +206,12 @@ Definition Client_reply_own (cl : loc) : iProp Σ :=
     "#Hlk" ∷ is_lock urpc_lockN #lk (Client_lock_inner Γ cl lk mref).
 
 (* TODO: move this *)
-Global Instance is_map_AsMapsTo mref hd :
-  AsMapsTo (map.is_map mref 1 hd) (λ q, map.is_map mref q hd).
+Global Instance own_map_AsMapsTo mref hd :
+  AsMapsTo (map.own_map mref 1 hd) (λ q, map.own_map mref q hd).
 Proof.
   split; try apply _; eauto.
   rewrite /fractional.Fractional.
-  rewrite /map.is_map.
+  rewrite /map.own_map.
   iIntros (p q). iSplit.
   - iDestruct 1 as (mv Heq) "H".
     iDestruct (fractional.fractional_split with "H") as "(H1&H2)".
@@ -226,12 +226,12 @@ Qed.
 
 Definition own_Server (s : loc) (handlers: gmap u64 val) : iProp Σ :=
   ∃ mref def,
-  "#Hhandlers_map" ∷ readonly (map.is_map mref 1 (handlers, def)) ∗
+  "#Hhandlers_map" ∷ readonly (map.own_map mref 1 (handlers, def)) ∗
   "#handlers" ∷ readonly (s ↦[Server :: "handlers"] #mref).
 
 Lemma wp_MakeServer (handlers : gmap u64 val) (mref:loc) (def : val) :
   {{{
-       map.is_map mref 1 (handlers, def)
+       map.own_map mref 1 (handlers, def)
   }}}
     MakeServer #mref @ ⊤
   {{{
@@ -295,7 +295,7 @@ Lemma wp_Server__readThread γ s host client handlers mref def :
   dom handlers ≠ ∅ →
   "#Hcomplete" ∷ handlers_complete γ handlers ∗
   "#His_rpc_map" ∷ urpc_handler_mapping γ host handlers ∗
-  "#Hhandlers_map" ∷ readonly (map.is_map mref 1 (handlers, def)) ∗
+  "#Hhandlers_map" ∷ readonly (map.own_map mref 1 (handlers, def)) ∗
   "#handlers" ∷ readonly (s ↦[Server :: "handlers"] #mref) -∗
   WP Server__readThread #s (connection_socket host client) {{ _, True }}.
 Proof.
