src/program_proof/memkv/memkv_shard_clerk_proof.v
@@ -67,7 +67,7 @@ Qed.
 
 Definition own_shard_phys kvs_ptr sid (kvs:gmap u64 (list u8)) : iProp Σ :=
   ∃ (mv:gmap u64 val),
-  "Hmap_phys" ∷ map.is_map kvs_ptr 1 (mv, (slice_val Slice.nil)) ∗
+  "Hmap_phys" ∷ map.own_map kvs_ptr 1 (mv, (slice_val Slice.nil)) ∗
   "%Hdom_phys" ∷ ⌜ dom kvs = dom mv ⌝ ∗
   ([∗ set] k ∈ (fin_to_set u64),
            (⌜shardOfC k ≠ sid ∧ mv !! k = None ∧ kvs !! k = None ⌝ ∨ (∃ q vsl, ⌜default (slice_val Slice.nil) (mv !! k) = (slice_val vsl)⌝ ∗ typed_slice.is_slice_small vsl byteT q (default [] (kvs !! k)))))
@@ -77,7 +77,7 @@ Definition own_shard_phys kvs_ptr sid (kvs:gmap u64 (list u8)) : iProp Σ :=
 Definition own_shard_phys kvs_ptr sid (kvs:gmap u64 (list u8)) : iProp Σ :=
   ∃ (mv:gmap u64 val),
   "%Hdom_phys" ∷ ⌜ dom mv = dom kvs ⌝ ∗
-  "Hmap_phys" ∷ map.is_map kvs_ptr 1 (mv, (slice_val Slice.nil)) ∗
+  "Hmap_phys" ∷ map.own_map kvs_ptr 1 (mv, (slice_val Slice.nil)) ∗
   "%Hdom_sid" ∷ ⌜ (∀ k, shardOfC k = sid → k ∈ dom mv) ⌝ ∗
   ([∗ map] k ↦ vsl' ∈ mv, ∃ q vsl, ⌜ vsl' = (slice_val vsl)⌝ ∗ typed_slice.is_slice_small vsl byteT q (default [] (kvs !! k))).
 *)
