src/program_proof/memkv/memkv_shard_make_proof.v
@@ -65,7 +65,7 @@ Proof.
                       own_shard γ.(kv_gn) sid m ∗ (* own shard *)
                       ⌜kvs_ptrs !! (int.nat sid) = Some kvs_ptr⌝ ∗
                       ⌜dom m = dom mv ⌝ ∗
-                      map.is_map kvs_ptr 1 (mv, (slice_val Slice.nil)) ∗
+                      map.own_map kvs_ptr 1 (mv, (slice_val Slice.nil)) ∗
                       ([∗ set] k ∈ (fin_to_set u64),
                        ⌜shardOfC k ≠ sid ∧ mv !! k = None ∧ m !! k = None⌝ ∨ (∃ q vsl, ⌜default (slice_val Slice.nil) (mv !! k) = (slice_val vsl)⌝ ∗ typed_slice.is_slice_small vsl byteT q (default [] (m !! k))))
                   )))%I with "[] [$Hi HshardMap_sl shardMap HghostShards kvss Hkvss_sl]").
